Semantics.thy
@@ -1,5 +1,15 @@
 theory Semantics imports Syntax "HOL-Library.AList" begin
 
+text\<open>For next meeting:
+Questions/Help:
+- Nominal2 proof for lookup_instance. Can't get the first goal to be solved.
+  Figured it was more productive to keep going for now.
+- Heaps, see text block below.
+To talk about:
+- Think I figured out what's going on with expression and formula semantics, see below.
+- See TODOs on the exp small-step semantics.
+- See TODO on exp.\<close>
+
 datatype heap = Heap "packet \<Rightarrow> bv" "instanc \<Rightarrow> bv option"
 
 text\<open>This is necessary to use heaps in nominal_functions. It basically states that
@@ -15,19 +25,24 @@ fun heap_lookup_packet :: "heap \<Rightarrow> packet \<Rightarrow> bv" where
 fun heap_lookup_instance :: "heap \<Rightarrow> instanc \<Rightarrow> bv option" where
   "heap_lookup_instance (Heap _ insts) i = insts i"
 
+(* Easier to work with than "var \<Rightarrow> heap" with Nominal2 because it has a finite support (I think) *)
 type_synonym env = "(var \<times> heap) list"
+
+(* These are declared in the LambdaAuth session, so I thought it might help *)
+declare
+  fresh_star_Pair[simp] fresh_star_insert[simp] fresh_Nil[simp]
+  pure_supp[simp] pure_fresh[simp]
 
 fun lookup_packet :: "env \<Rightarrow> var \<Rightarrow> packet \<Rightarrow> bv option" where
   "lookup_packet \<epsilon> x p = map_option (\<lambda>h. heap_lookup_packet h p) (map_of \<epsilon> x)"
 fun lookup_instance :: "env \<Rightarrow> var \<Rightarrow> instanc \<Rightarrow> bv option" where
   "lookup_instance \<epsilon> x i = Option.bind (map_of \<epsilon> x) (\<lambda>h. heap_lookup_instance h i)"
-(* This also doesn't work because sliceable is a nominal_datatype atm... *)
 nominal_function lookup_sliceable :: "sliceable \<Rightarrow> env \<Rightarrow> bv option" where
   "lookup_sliceable (SlPacket x p) \<epsilon> = lookup_packet \<epsilon> x p" |
   "lookup_sliceable (SlInstance x i) \<epsilon> = lookup_instance \<epsilon> x i"
-  using [[simproc del: alpha_lst]]
-  subgoal unfolding eqvt_def by (auto simp add: lookup_sliceable_graph_aux_def permute_heap_def
-                                            permute_list_def permute_option_def permute_bool_def permute_char_def)
+sorry
+(*  using [[simproc del: alpha_lst defined_all]]
+  subgoal by (simp add: eqvt_def lookup_sliceable_graph_aux_def)
   subgoal by (erule lookup_sliceable_graph.induct) (auto simp: fresh_star_def fresh_at_base)
                       apply clarify
   subgoal for P t s y
@@ -40,26 +55,84 @@ nominal_function lookup_sliceable :: "sliceable \<Rightarrow> env \<Rightarrow> 
     apply (metis fresh_star_def fresh_star_supp_conv supp_perm_eq_test)
     apply (metis fresh_star_def fresh_star_supp_conv supp_perm_eq_test)
     done
-  done
+  done*)
 nominal_termination (eqvt)
   by lexicographic_order
 
 term lookup_sliceable_graph_aux
 
-datatype val = BV bv | Num nat
-
 fun slice :: "'a list \<Rightarrow> int \<Rightarrow> int \<Rightarrow> 'a list" where
   "slice xs n m = take (nat (m - n)) (drop (nat n) xs)"
 
-text\<open>It seems I can't define the semantics here as a function (which would be closer to how the
-paper presents it. Is this a limitation of Nominal2? Am I using it wrong?\<close>
-(*
-nominal_function exp_sem :: "exp \<Rightarrow> val option" where
-  "exp_sem (Len x p) = map_option (\<lambda>h. Num (length (heap_lookup_packet h p))) (\<epsilon> x)"
+
+text\<open>About the semantics for expressions and formulas...
+The paper references, but never defines, small-step semantics for formulas and expressions, which
+are used to define the command small-step semantics and prove the corresponding type safety theorems.
+These are shown to be of the form "(I, O, H, e) -> e'", basically the same form as for commands. H
+here is "a map that relates instance names to records containing the field values". Expressions
+referring to a variable always refer to an implicit variable "heap" when used in commands, which
+corresponds with the H parameter for the small-step semantics.
+
+What the paper does present are denotational-style semantics for a subset of expressions. It also
+defines them for formulas (in the text below Fig. 5). These are both defined in terms of an
+environment \<epsilon> that maps variable names to heaps, that is also used to define the semantics of
+heap *types*.
+
+So, right now my assumption is that we'll need both: small-step semantics to define small-step
+command semantics and ideally denotational semantics / a function to define the semantics of heap
+types (especially refinement types). Unless we can use of them for both? (e.g. use the small-step
+ones for types too?) Probably not because of the different environments I think.
+\<close>
+
+text\<open>Relatedly, let's talk about heaps.
+Section 3.3 says "We model heaps as maps from names to bit vectors".
+
+Section 3.4 says "H is a map that relates instance names to records containing the field values"
+(where H is one of the arguments for the small-step judgement). Later (in appendix B) (I, O, H) is
+defined to mean H[PktIn -> I, PktOut -> O] which is a heap, as defined above. This seems to apply
+that H really maps instance names to bit vectors too?
+I suppose technically there is a 1-to-1 correspondence between a full instance bit vector and a
+"record containing the field values" for an instance. But do we really have to model it like this,
+converting back and forth when needed?
+\<close>
+
+(* TODO: At the moment, we just ignore variables here and assume they must be "heap". Should we
+   explicitly encode that in the rule assumptions? *)
+(* TODO: Which of these is preferable?
+    E_PktIn:      "(In, Out, H, Packet x PktIn) \<rightarrow> Bv In" |
+    E_PktIn:      "\<lbrakk> p = PktIn \<rbrakk> \<Longrightarrow> (In, Out, H, Packet x p) \<rightarrow> Bv In" |
+  and similarly, keep len call in the rule or make it a premise in E_Pkt*Len?
 *)
+inductive
+  exp_small_step :: "(bv \<times> bv \<times> headers \<times> exp) \<Rightarrow> exp \<Rightarrow> bool" ("_ \<rightarrow>/ _" [0,50] 50)
+where
+  E_Plus1:      "\<lbrakk> (In, Out, H, e\<^sub>1) \<rightarrow> e\<^sub>1' \<rbrakk>
+                \<Longrightarrow> (In, Out, H, Plus e\<^sub>1 e\<^sub>2) \<rightarrow> Plus e\<^sub>1' e\<^sub>2" |
+  E_Plus2:      "\<lbrakk> value v\<^sub>1; (In, Out, H, e\<^sub>2) \<rightarrow> e\<^sub>2' \<rbrakk>
+                \<Longrightarrow> (In, Out, H, Plus v\<^sub>1 e\<^sub>2) \<rightarrow> Plus v\<^sub>1 e\<^sub>2'" |
+  E_Plus:       "\<lbrakk> v\<^sub>1 = Num n\<^sub>1; v\<^sub>2 = Num n\<^sub>2 \<rbrakk>
+                \<Longrightarrow> (In, Out, H, Plus v\<^sub>1 v\<^sub>2) \<rightarrow> Num (n\<^sub>1 + n\<^sub>2)" |
+  E_Concat1:    "\<lbrakk> (In, Out, H, e\<^sub>1) \<rightarrow> e\<^sub>1' \<rbrakk>
+                \<Longrightarrow> (In, Out, H, Concat e\<^sub>1 e\<^sub>2) \<rightarrow> Concat e\<^sub>1 e\<^sub>2" |
+  E_Concat2:    "\<lbrakk> value v\<^sub>1; (In, Out, H, e\<^sub>2) \<rightarrow> e\<^sub>2' \<rbrakk>
+                \<Longrightarrow> (In, Out, H, Concat v\<^sub>1 e\<^sub>2) \<rightarrow> Concat v\<^sub>1 e\<^sub>2'" |
+  E_Concat:     "\<lbrakk> v\<^sub>1 = Bv b\<^sub>1; v\<^sub>2 = Bv b\<^sub>2 \<rbrakk>
+                \<Longrightarrow> (In, Out, H, Concat v\<^sub>1 v\<^sub>2) \<rightarrow> Bv (b\<^sub>1 @ b\<^sub>2)" |
+  E_PktIn:      "(In, Out, H, Packet x PktIn) \<rightarrow> Bv In" |
+  E_PktOut:     "(In, Out, H, Packet x PktOut) \<rightarrow> Bv Out" |
+  E_PktInLen:   "(In, Out, H, Len x PktIn) \<rightarrow> Num (len In)" |
+  E_PktOutLen:  "(In, Out, H, Len x PktOut) \<rightarrow> Num (len Out)" |
+  (*E_Slice1:     "\<lbrakk> (In, Out, H, e\<^sub>1) \<rightarrow> e\<^sub>1' \<rbrakk>
+                \<Longrightarrow> (In, Out, H, Slice sl e\<^sub>1 e\<^sub>2) \<rightarrow> Slice sl e\<^sub>1' e\<^sub>2" |
+  E_Slice2:     "\<lbrakk> value v\<^sub>1; (In, Out, H, e\<^sub>2) \<rightarrow> e\<^sub>2' \<rbrakk>
+                \<Longrightarrow> (In, Out, H, Slice sl v\<^sub>1 e\<^sub>2) \<rightarrow> Slice sl v\<^sub>1 e\<^sub>2'" | *)
+  E_SlicePktIn: "\<lbrakk> 0 \<le> n \<and> n < m \<and> m \<le> (len In + 1); slice In n m = bs \<rbrakk>
+                \<Longrightarrow> (In, Out, H, Slice (SlPacket x PktIn) n m) \<rightarrow> Bv bs" |
+  E_SlicePktOut:"\<lbrakk> 0 \<le> n \<and> n < m \<and> m \<le> (len Out + 1); slice Out n m = bs \<rbrakk>
+                \<Longrightarrow> (In, Out, H, Slice (SlPacket x PktOut) n m) \<rightarrow> Bv bs" |
+  E_SliceInst:  "\<lbrakk> H \<rbrakk>
+                \<Longrightarrow> (In, Out, H, Slice (SlInstance x i) n m) \<rightarrow> Num 0"
 
-
-text\<open>These are the expression semantics as an inductive predicate instead for now:\<close>
 inductive exp_sem :: "exp \<Rightarrow> env \<Rightarrow> val \<Rightarrow> bool" where
   "exp_sem (Syntax.Num n) _ (Num n)" |
   "exp_sem (Bv bs) _ (BV bs)" |
@@ -79,18 +152,12 @@ inductive form_sem :: "formula \<Rightarrow> env \<Rightarrow> bool \<Rightarrow
   "\<lbrakk> exp_sem e\<^sub>1 \<epsilon> (Num n\<^sub>1); exp_sem e\<^sub>2 \<epsilon> (Num n\<^sub>2); n\<^sub>1 \<le> n\<^sub>2 \<rbrakk> \<Longrightarrow> form_sem (Gt e\<^sub>1 e\<^sub>2) \<epsilon> false"
   (*"\<lbrakk> exp_sem e\<^sub>1 \<epsilon> (Num n\<^sub>1); exp_sem e\<^sub>2 \<epsilon> (Num n\<^sub>2); n\<^sub>1 \<le> n\<^sub>2 \<rbrakk> \<Longrightarrow> form_sem (And e\<^sub>1 e\<^sub>2) \<epsilon> false"*)
 
-
-
-type_synonym header_instance = "string \<Rightarrow> bv"
-type_synonym headers = "instanc \<Rightarrow> header_instance"
-
 (*datatype cmd =
   Extract instanc | Remit instanc | Add instanc |
   If formula cmd cmd | Seq cmd cmd | Assign instanc string exp |
   Skip | Reset | Ascribe cmd pi_ty
 *)
 
-(* TODO: Is it possible to use O as variable name? Leads to a parse error if I try. *)
 (* I added HT as the extra ambient/global context explicitly here. *)
 inductive
   small_step :: "header_table \<Rightarrow> (bv \<times> bv \<times> headers \<times> cmd) \<Rightarrow> (bv \<times> bv \<times> headers \<times> cmd) \<Rightarrow> bool"
